working on bounding theorems

impls_with_Z.v
@@ -7,6 +7,7 @@ Require Import ZNatPairs.
 Require Import Zsqrt.
 Require Import R_Ifp.
 Require Import Even.
+Require Import Znat.
 
 Open Scope Z_scope.
 
@@ -72,6 +73,15 @@ Lemma consec_mult__even : forall (w : Z),
 (Zeven (w * (w + 1))).
 Proof.
 intro w.
+destruct (Zeven_odd_dec w) as [E | O].
+
+SearchAbout Zeven.
+
+apply Zeven_ex in E.
+destruct E as [m EQ].
+subst w.
+(* apply Zeven_2p. *)
+
 Admitted.
 
 Lemma refactor_sqr_term : forall w,
@@ -97,74 +107,111 @@ w >= 0 ->
 0 <= 2 * w + 1.
 Proof.
 intros w w_pos.
-Admitted.
+omega.
+Qed.
 
 Theorem w_Result_Z_int : forall w t,
   w >= 0 ->
   t = Zdiv2 (w * (w + 1)) ->
   w_Result_Z w t.
 Proof.
-intros w t w_positive t_def. subst. 
-unfold w_Result_Z. unfold Result_Z.
+  intros w t w_positive t_def. subst. 
+  unfold w_Result_Z. unfold Result_Z.
 
-assert (
+  assert (
         Zdiv2 (Zsqrt_plain (8 * Zdiv2 (w * (w + 1)) + 1) - 1) =
         Zdiv2 (Zsqrt_plain (4*2*Zdiv2 (w * (w + 1)) + 1) - 1)).
-reflexivity.
-rewrite -> H. clear H.
+  reflexivity.
+  rewrite -> H. clear H.
 
 
-rewrite <- Zmult_assoc.
-rewrite <- Zeven_div2.
+  rewrite <- Zmult_assoc.
+  rewrite <- Zeven_div2.
 
-rewrite refactor_sqr_term.
-remember (2 * w + 1) as sqr_term.
+  rewrite refactor_sqr_term.
+  remember (2 * w + 1) as sqr_term.
 
-rewrite Zsqrt_square_id.
+  rewrite Zsqrt_square_id.
 
-rewrite Heqsqr_term.
+  rewrite Heqsqr_term.
 
-rewrite plus_minus_assoc.
-rewrite (Zminus_diag 1).
-rewrite Zplus_0_r.
+  rewrite plus_minus_assoc.
+  rewrite (Zminus_diag 1).
+  rewrite Zplus_0_r.
 
-apply Zdiv2_Zmult2.
+  apply Zdiv2_Zmult2.
 
-rewrite Heqsqr_term.
-apply sqr_term_positive. exact w_positive.
+  rewrite Heqsqr_term.
+  apply sqr_term_positive. exact w_positive.
 
-apply consec_mult__even.
+  apply consec_mult__even.
 Qed.
 
+(*
+define decreasing
+increasing f -> n <= m <-> f n <= f m
+increasing result
+therefore n <= m -> result n <= result m
+*)
+
+Definition increasing f : Prop := forall x y, x <= y -> f x <= f y.
+
+Lemma Result_Z_increasing :
+increasing Result_Z.
+Proof.
+  unfold increasing.
+  intros.
+  unfold Result_Z.
+  assert (increasing Zdiv2). admit.
+  apply H0.
+  assert (increasing Zsqrt_plain). admit.
+  assert (increasing (fun x => x - 1)). admit.
+  apply H2. apply H1. omega.
+Qed.
+  
 
 (* t <= z < t + w + 1  ->
    w <= Result z < w + 1  *)
 Theorem z_bounds : forall (w t z : Z),
- Zle t z -> Zlt z (t + w + 1) ->
- Zle w (Result_Z z) -> Zlt (Result_Z z) (w + 1).
+ w_Result_Z w t ->
+ t <= z -> z < (t + w + 1) ->
+ w <= (Result_Z z) < (w + 1).
 Proof.
-  intros.
-  unfold Result_Z.
+  intros w t z H1 H2 H3.
+  split.
+  unfold w_Result_Z in H1. subst w.
+  assert (increasing Result_Z).
+  apply Result_Z_increasing.
+  apply H. exact H2.
+
+  unfold w_Result_Z in H1.
+  subst w.
 Admitted.
+
+Definition Zfloor (x : R) := (up x - 1)%Z.
 
 (* w <= Result z < w + 1  ->
    w = floor (Result z)  *)
 Theorem w__floor_Result_Z : forall (w z : Z),
   Zle w (Result_Z z) -> Zlt (Result_Z z) (w + 1) ->
-  w = Int_part (Result z).
+  w = Zfloor (Result z).
 Proof.
+  intros w z H1 H2.
+  unfold Zfloor.
+  (* change definitions to Zfloor instead of Int_part! *)
 Admitted.
 
 
 Theorem decode_encode : forall x y ,
     decode (encode (x, y)) = (x, y).
 Proof.
- intros x y.
+  intros x y.
 Admitted.
 
 Theorem encode_decode : forall z ,
     encode (decode z) = z.
 Proof.
+  intros. unfold decode. unfold encode. simpl.
 Admitted.
 
 Close Scope Z_scope.
